Experiment with live sets in memory safety.

memory_safety/propertyA.v
@@ -1,7 +1,9 @@
 Require Import Ssreflect.ssreflect Ssreflect.ssrfun Ssreflect.ssrbool.
-Require Import Ssreflect.ssrnat Ssreflect.seq Ssreflect.eqtype.
+Require Import Ssreflect.ssrnat Ssreflect.seq Ssreflect.eqtype Ssreflect.fintype.
 
-Require Import CoqUtils.ord CoqUtils.word CoqUtils.partmap.
+Require Import MathComp.path MathComp.fingraph.
+
+Require Import CoqUtils.ord CoqUtils.word CoqUtils.partmap CoqUtils.fset.
 
 Require Import lib.utils common.types.
 Require Import memory_safety.property memory_safety.abstract.
@@ -20,8 +22,67 @@ Variable block : ordType.
 Variable allocator : Abstract.allocator mt block.
 Variable addrs : memory_syscall_addrs mt.
 
+Hypothesis allocatorP : Abstract.allocator_spec allocator.
+
 Local Notation state := (Abstract.state mt block).
 Local Notation pointer := [eqType of Abstract.pointer mt block].
+
+Implicit Type s : state.
+Implicit Type b : block.
+Implicit Type p : pointer.
+Implicit Type bs : {fset block}.
+
+Definition references s b b' :=
+  [exists offs : mword mt * mword mt,
+    Abstract.getv (Abstract.mem s) (b, offs.1) ==
+    Some (Abstract.VPtr (b', offs.2))].
+
+Inductive reachable s b : Prop :=
+| ReachBase r off of Abstract.regs s r = Some (Abstract.VPtr (b, off))
+| ReachHop b' of reachable s b' & references s b' b.
+
+Definition live_blocks s bs :=
+  (forall b, b \in bs <-> reachable s b) /\
+  (forall b, b \in bs -> b \in Abstract.blocks s).
+
+CoInductive valid_write s s' bs : Prop :=
+| ValidWrite p v
+  of Abstract.updv (Abstract.mem s) p v = Some (Abstract.mem s')
+  &  p.1 \in bs.
+
+CoInductive valid_free s s' bs : Prop :=
+| ValidFree b
+  of Abstract.free_fun (Abstract.mem s) b = Some (Abstract.mem s')
+  &  b \in bs.
+
+Ltac contradict_equal_mem :=
+  match goal with
+  | H : is_true (?x != ?x) |- _ => by rewrite eqxx in H
+  end.
+
+Lemma change_no_alloc s s' bs :
+  Abstract.step s s' ->
+  live_blocks s bs ->
+  live_blocks s' bs ->
+  Abstract.mem s != Abstract.mem s' ->
+  valid_write s s' bs \/ valid_free s s' bs.
+Proof.
+case: s s' / => /=; try (move=> *; contradict_equal_mem).
+- move=> m m' rs b pc ptr i r1 r2 v _ _ get_ptr _ upd_m [hbs _] _ _.
+  left; econstructor; eauto.
+  apply/hbs; apply/(@ReachBase _ ptr.1 r1 ptr.2); simpl; eauto.
+  by case: {upd_m get_ptr} ptr get_ptr.
+- move=> m m' rs rs' bs' sz b pc' _ hm' hrs' _ [/= /(_ b) hbs /(_ b) hsub]
+         [/= /(_ b) hbs' /(_ b) hsub'] _.
+  generalize (Abstract.malloc_fresh hm'); rewrite hsub //; apply/hbs'.
+  apply: (@ReachBase _ _ syscall_ret 0%w) => /=.
+  by rewrite (updm_set hrs') getm_set eqxx.
+move=> m m' r ptr bs' pc' harg hm' _ [hbs1 _] hbs2 _.
+right; eapply ValidFree; simpl; first by eauto.
+apply/hbs1.
+eapply (@ReachBase _ _ syscall_arg1 ptr.2); simpl; eauto.
+case: ptr harg {hm'} => /=; eauto.
+Qed.
 
 Definition get_events (s : state) : seq (event pointer block) :=
   match Abstract.pc s with
